Add hoare triple for State and lemmas, try exemples

Monads.v
@@ -6,7 +6,7 @@ Import Notations.
 
 Local Notation "f ∘ g" := (fun x => f (g x)) (at level 40, left associativity).
 
-Section definition.
+(* Section definition. *)
 
 Class Monad (m: Type -> Type) :=
 { return_ : forall {A}, A -> m A;
@@ -39,10 +39,14 @@ Class MonadTrans {m} `{Monad m} (t : (Type -> Type) -> (Type -> Type)) `{Monad(t
  (*  getT : get *)
 }.
 
-End definition.
+Notation "m1 ;; m2" := (bind m1 (fun _ => m2))  (at level 60, right associativity) : monad_scope.
+Notation "'perf' x '<-' m ';' e" := (bind m (fun x => e))
+  (at level 60, x ident, m at level 200, e at level 60) : monad_scope.
+
+(* End definition. *)
 
 
-Notation "a >>= f" := (bind a f) (at level 50, left associativity) : monad_scope.
+(* Notation "a >>= f" := (bind a f) (at level 50, left associativity) : monad_scope. *)
 Open Scope monad_scope.
 Arguments Monad m : assert.
 
@@ -135,8 +139,109 @@ Global Program Instance stateM : Monad (State) :=
   reflexivity.
   Qed.
 
-Definition HoareTripleS {A} (P : S -> Prop) (m : State A) (Q : A -> S -> Prop) : Prop :=
+Definition Assertion := S -> Prop.
+
+Definition hoareTripleS {A} (P : S -> Prop) (m : State A) (Q : A -> S -> Prop) : Prop :=
   forall (s : S), P s -> let (a, s') := m s in Q a s'.
+
+Notation "{{ P }} m {{ Q }}" := (hoareTripleS P m Q)
+  (at level 90, format "'[' '[' {{  P  }}  ']' '/  ' '[' m ']' '['  {{  Q  }} ']' ']'") : monad_scope.
+
+Lemma l_ret (A : Type) `{State A} (a : A) (P : A -> Assertion) : {{ P a }} return_ a {{ P }}.
+Proof.
+intros s H; trivial.
+Qed.
+
+(* Triplet de hoare sur la séquence *)
+Lemma l_bind  (A B : Type) (m : State A) (f : A -> State B) (P : Assertion)( Q : A -> Assertion) (R : B -> Assertion) :
+  (forall a, {{ Q a }} f a {{ R }}) -> {{ P }} m {{ Q }} -> {{ P }} perf x <- m ; f x {{ R }}.
+Proof. 
+intros H1 H2 s H3.
+unfold state_bind.
+case_eq (m s).
+intros.
+apply H2 in H3.
+case_eq (f a s0).
+intros b s'' H5.
+Admitted.
+
+Definition wp {A : Type} (P : A -> S -> Prop) (m : State A) :=
+  fun s => let (a,s') := m s in P a s'.
+
+Lemma wpIsPrecondition {A : Type} (P : A -> S -> Prop) (m : State A) :
+  {{ wp P m }} m {{ P }}.
+  Proof.
+  unfold wp.
+  congruence.
+  Qed.
+
+Lemma wpIsWeakestPrecondition
+  (A : Type) (P : A -> S -> Prop) (Q : S -> Prop) (m : State A) :
+  {{ Q }} m {{ P }} -> forall s, Q s -> (wp P m) s.
+  Proof.
+  trivial.
+  Qed.
+
+Lemma assoc (A B C : Type)(m : State A)(f : A -> State B)(g : B -> State C) :
+  perf y <-
+    perf x <- m ;
+    f x ;
+  g y =
+  perf x <- m ;
+  perf y <- f x ;
+  g y.
+  Proof.
+  extensionality s.
+  unfold bind.
+  case (m s).
+  simpl.
+  intros.
+  unfold state_bind.
+  case (m s).
+  intros.
+  reflexivity.
+  Qed.
+
+Definition modify (f : S -> S) : State () :=
+  getS >>= (fun s => putS (f s)).
+
+Lemma l_put (s : S) (P : unit -> Assertion) : {{ fun _ => P tt s }} putS s {{ P }}.
+Proof.
+intros s0 H;trivial.
+Qed.
+
+Lemma l_get (P : S -> Assertion) : {{ fun s => P s s }} getS {{ P }}.
+Proof.
+intros s H; trivial.
+Qed.
+
+Lemma bindRev (A B : Type) (m : State A) (f : A -> State B) (P : Assertion)( Q : A -> Assertion) (R : B -> Assertion) :
+  {{ P }} m {{ Q }} -> (forall a, {{ Q a }} f a {{ R }}) -> {{ P }} perf x <- m ; f x {{ R }}.
+Proof.
+intros; eapply l_bind ; eassumption.
+Qed.
+
+Lemma weaken (A : Type) (m : State A) (P Q : Assertion) (R : A -> Assertion) :
+  {{ Q }} m {{ R }} -> (forall s, P s -> Q s) -> {{ P }} m {{ R }}.
+Proof.
+intros H1 H2 s H3.
+apply H2 in H3. 
+apply H1 in H3.
+assumption. 
+Qed.
+
+Lemma l_modify f (P : () -> Assertion) : {{ fun s => P tt (f s) }} modify f {{ P }}.
+Proof.
+unfold modify.
+eapply l_bind.
+intros.
+eapply l_put.
+simpl.
+eapply weaken.
+eapply l_get.
+intros. simpl.
+assumption.
+Qed.
 
 (* Global Instance stateS : MonadState (State) :=
   {  get := @getS;
@@ -144,9 +249,6 @@ Definition HoareTripleS {A} (P : S -> Prop) (m : State A) (Q : A -> S -> Prop) :
     run := @runState;
   }. *)
 (*     hoareTriple : @ *)
-
-Definition modify (f : S -> S) : State unit :=
-  getS >>= (fun s => putS (f s)).
 
 End monadic_state.
 
@@ -255,11 +357,8 @@ stepLoopT body (fun _ => return_ tt).
 
 End monadic_loop.
 
-Notation "m1 ;; m2" := (bind m1 (fun _ => m2))  (at level 60, right associativity) : monad_scope.
-Notation "'perf' x '<-' m ';' e" := (bind m (fun x => e))
-  (at level 60, x ident, m at level 200, e at level 60) : monad_scope.
 Notation "'for' i '=' min 'to' max '{{' body }}" := (foreach' min max (fun i => (loopT_liftT body))) (at level 60, i ident, min at level 60,
 max at level 60, body at level 60, right associativity) : monad_scope.
 
-Notation "'fore' i '=' min 'to' max '{{' body }}" := (foreach' min max (fun i => (body))) (at level 60, i ident, min at level 60,
+Notation "'for_e' i '=' min 'to' max '{{' body }}" := (foreach' min max (fun i => (body))) (at level 60, i ident, min at level 60,
 max at level 60, body at level 60, right associativity) : monad_scope.
