Prog.v
@@ -1,4 +1,4 @@
-Require Import Monads List ZArith.
+Require Import Monads List ZArith Program.
 
 Open Scope monad_scope.
 
@@ -18,17 +18,62 @@ Definition add_s (i : nat) : Monads.State nat unit :=
 Definition minus_s (i : nat) : Monads.State nat unit :=
   Monads.modify (fun s => s - i).
 
-Definition getVal : State nat nat:= return_ 10.
+Definition get10 : State nat nat:= return_ 10.
 
-Compute runState (
-  for i = 0 to 3 {{ 
+Definition count15 : State nat unit :=
+ add_s 1;;
+ add_s 2;;
+ add_s 3;;
+ add_s 4;;
+ add_s 5;;
+ return_ tt.
+
+Notation "{{ P }} m {{ Q }}" := (hoareTripleS P m Q)
+  (at level 90, format "'[' '[' {{  P  }}  ']' '/  ' '[' m ']' '['  {{  Q  }} ']' ']'") : monad_scope.
+
+SearchAbout Nat.add.
+
+Lemma l_add_s :
+ forall (n i : nat), {{fun (s : nat) => s = n}} add_s i {{fun (_ : unit) (s : nat) => s = n + i}}.
+  Proof.
+  intros n i s H.
+  unfold add_s.
+  apply l_modify.
+  auto.
+  Qed.
+
+Lemma l_count15 : {{fun s : nat => s = init_S1}} count15 {{fun (_ : unit ) (s : nat) => s = 15}}.
+  Proof.
+  apply bindRev with (Q := (fun (_ : unit ) (s : nat) => s = 1)); try apply l_add_s.
+  + intros; apply bindRev with (Q := (fun (_ : unit ) (s : nat) => s = 3)) ; try apply l_add_s.
+  - intros; apply bindRev with (Q := (fun (_ : unit ) (s : nat) => s = 6)) ; try apply l_add_s.
+  * intros; apply bindRev with (Q := (fun (_ : unit ) (s : nat) => s = 10)) ; try apply l_add_s.
+    intros; apply bindRev with (Q := (fun (_ : unit ) (s : nat) => s = 15)) ; try apply l_add_s.
+    intros. intros S H. trivial.
+  Qed.
+
+Definition count42 : State nat unit
+ := for i = 0 to 3 {{ 
     add_s i ;;
     add_s i ;;
-    perf x <- getVal;
+    perf x <- get10;
     add_s x ;;
     add_s i ;;
     add_s i
-  }} 
+  }} .
+
+Lemma l_count42 : hoareTripleS (fun s : nat => s = init_S1) count42 (fun (_ : unit ) (s : nat) => s = 42).
+  Proof.
+  eapply bindRev.
+  unfold count42.
+  unfold loopT_liftT.
+  eapply bindRev.
+  Qed.
+
+Check count42.
+
+Compute runState (
+  count42
   ) init_S1.
 
 Compute runState (
